ModelChecking_sol.v
@@ -1,0 +1,82 @@
+Theorem factorial_ok_2 :
+  invariantFor (factorial_sys 2) (fact_correct 2).
+Proof.
+  simplify.
+  eapply invariant_weaken.
+  (* We begin like in last chapter, by strengthening to an inductive
+   * invariant. *)
+
+  apply multiStepClosure_ok.
+  (* The difference is that we will use multi-step closure to find the invariant
+   * automatically.  Note that the invariant appears as an existential variable,
+   * whose name begins with a question mark. *)
+  simplify.
+  rewrite fact_init_is.
+  (* It's important to phrase the current candidate invariant explicitly as a
+   * finite set, before continuing.  Otherwise, it won't be obvious how to take
+   * the one-step closure. *)
+
+  (* Compute which states are reachable after one step. *)
+  eapply MscStep.
+  apply oneStepClosure_split; simplify.
+  invert H; simplify.
+  apply singleton_in.
+  apply oneStepClosure_empty.
+  simplify.
+
+  (* Compute which states are reachable after two steps. *)
+  eapply MscStep.
+  apply oneStepClosure_split; simplify.
+  invert H; simplify.
+  apply singleton_in.
+  apply oneStepClosure_split; simplify.
+  invert H; simplify.
+  apply singleton_in.
+  apply oneStepClosure_empty.
+  simplify.
+
+  (* Compute which states are reachable after three steps. *)
+  eapply MscStep.
+  apply oneStepClosure_split; simplify.
+  invert H; simplify.
+  apply singleton_in.
+  apply oneStepClosure_split; simplify.
+  invert H; simplify.
+  apply singleton_in.
+  apply oneStepClosure_split; simplify.
+  invert H; simplify.
+  apply singleton_in.
+  apply oneStepClosure_empty.
+  simplify.
+
+  (* Now the candidate invariatn is closed under single steps.  Let's prove
+   * it. *)
+  apply MscDone.
+  apply prove_oneStepClosure; simplify.
+  propositional.
+  propositional; invert H0; try equality.
+  invert H; equality.
+  invert H1; equality.
+
+  (* Finally, we prove that our new invariant implies the simpler, noninductive
+   * one that we started with. *)
+  simplify.
+  propositional; subst; simplify; propositional.
+  (* [subst]: remove all hypotheses like [x = e] for variables [x], simply
+   *   replacing all uses of [x] by [e]. *)
+Qed.
+
+Theorem twoadd2_ok :
+  invariantFor (parallel twoadd_sys twoadd_sys) (twoadd_correct (private := _)).
+Proof.
+  eapply invariant_weaken.
+  eapply invariant_simulates.
+  apply withInterference_abstracts.
+  apply withInterference_parallel.
+  apply twoadd_ok.
+  apply twoadd_ok.
+
+  unfold twoadd_correct.
+  invert 1.
+  assumption.
+Qed.
